src/dafny/ssz/Serialise.dfy
@@ -14,11 +14,13 @@
 
 
 include "../utils/NativeTypes.dfy"
+include "../utils/NonNativeTypes.dfy"
 include "../utils/Eth2Types.dfy"
 include "../utils/Helpers.dfy"
 include "IntSeDes.dfy"
 include "BoolSeDes.dfy"
 include "BitListSeDes.dfy"
+include "../utils/MathHelpers.dfy"
 
 /**
  *  SSZ library.
@@ -28,11 +30,13 @@ include "BitListSeDes.dfy"
 module SSZ {
 
     import opened NativeTypes
+    import opened NonNativeTypes
     import opened Eth2Types
     import opened IntSeDes
     import opened BoolSeDes
     import opened BitListSeDes
     import opened Helpers
+    import opened MathHelpers
 
     /** SizeOf.
      *
@@ -43,14 +47,24 @@ module SSZ {
      *              i.e. uintN or bool.
      */
     function method sizeOf(s: Serialisable): nat
-        requires || typeOf(s) == Bool_
-                 || exists n:nat :: typeOf(s) == Uint_(n)
+        requires typeOf(s) in {Bool_, Uint8_, Uint16_, Uint32_, Uint64_, Uint128_, Uint256_}
         ensures 1 <= sizeOf(s) <= 32
         ensures sizeOf(s) == |serialise(s)|
     {
         match s
             case Bool(_) => 1
-            case Uint(n) => n.byteLength
+
+            case Uint8(_) => 1
+
+            case Uint16(_) => 2
+
+            case Uint32(_) => 4
+
+            case Uint64(_) => 8
+
+            case Uint128(_) => 16
+
+            case Uint256(_) => 32
     }
 
     /** default.
@@ -60,13 +74,22 @@ module SSZ {
      *
     */
     function method default(t : Tipe) : Serialisable 
-    requires || t in {Bool_,Bitlist_,Bytes32_}
-             || exists n:nat :: t == Uint_(n)
+    requires t in {Bool_, Uint8_, Uint16_, Uint32_, Uint64_, Uint128_, Uint256_, Bitlist_,Bytes32_}
     {
             match t 
                 case Bool_ => Bool(false)
         
                 case Uint_(_) => Uint(Uint256WithByteLength(0,1))
+
+                case Uint16_ => Uint16(0)
+
+                case Uint32_ => Uint32(0)
+
+                case Uint64_ => Uint64(0)
+
+                case Uint128_ => Uint128(0)
+
+                case Uint256_ => Uint256(0)                
 
                 case Bitlist_ => Bitlist([])
 
@@ -79,13 +102,25 @@ module SSZ {
      *  @returns    A sequence of bytes encoding `s`.
      */
     function method serialise(s : Serialisable) : seq<byte> 
-    requires || typeOf(s) in {Bool_,Bitlist_,Bytes32_}
-             || exists n:nat :: typeOf(s) == Uint_(n)
+    requires typeOf(s) in {Bool_, Uint8_, Uint16_, Uint32_, Uint64_, Uint128_, Uint256_, Bitlist_, Bytes32_}
     {
         match s
             case Bool(b) => boolToBytes(b)
 
-            case Uint(n) => uintToBytes(s)
+            case Uint8(n) => int_to_bytes(s.n8 as nat, 1)
+
+            case Uint16(n) => int_to_bytes(s.n16 as nat, 2)
+
+            case Uint32(n) => int_to_bytes(s.n32 as nat, 4)
+
+            case Uint64(n) =>   UpperBoundForUint64(s.n64);
+                                assert 64 == 8 * 8;
+                                int_to_bytes(s.n64 as nat, 8)
+
+            case Uint128(n) =>  assert 128 == 16 * 8;
+                                int_to_bytes(s.n128 as nat, 16)
+
+            case Uint256(n) => int_to_bytes(s.n256 as nat, 32)         
 
             case Bitlist(xl) => fromBitlistToBytes(xl)
 
@@ -103,8 +138,7 @@ module SSZ {
      *              that has not been used in the deserialisation as well.
      */
     function method deserialise(xs : seq<byte>, s : Tipe) : Try<Serialisable>
-    requires || s in {Bool_,Bitlist_,Bytes32_}
-             || exists n:nat :: s == Uint_(n)
+    requires s in {Bool_, Uint8_, Uint16_, Uint32_, Uint64_, Uint128_, Uint256_, Bitlist_,Bytes32_}
     {
         match s
             case Bool_ => if |xs| == 1 then
@@ -112,10 +146,35 @@ module SSZ {
                             else 
                                 Failure
                             
-            case Uint_(byteLength) =>   if 1 <= |xs| == byteLength <= 32 then
-                                            Success(byteToUint(xs))
-                                        else 
-                                            Failure
+            case Uint8_ =>   if |xs|  == sizeOf(default(s)) then
+                                Success(Uint8(bytes_to_int(xs) as uint8))
+                            else 
+                                Failure
+
+            case Uint16_ =>   if |xs|  == sizeOf(default(s)) then
+                                Success(Uint16(bytes_to_int(xs) as uint16))
+                            else 
+                                Failure
+
+            case Uint32_ =>   if |xs|  == sizeOf(default(s)) then
+                                Success(Uint32(bytes_to_int(xs) as uint32))
+                            else 
+                                Failure
+
+            case Uint64_ =>   if |xs|  == sizeOf(default(s)) then
+                                Success(Uint64(bytes_to_int(xs) as uint64))
+                            else 
+                                Failure
+
+            case Uint128_ =>   if |xs|  == sizeOf(default(s)) then
+                                Success(Uint128(bytes_to_int(xs) as uint128))
+                            else 
+                                Failure
+
+            case Uint256_ =>   if |xs|  == sizeOf(default(s)) then
+                                Success(Uint256(bytes_to_int(xs) as uint256))
+                            else 
+                                Failure                                                                                                                                                                
                                 
             case Bitlist_ => if (|xs| >= 1 && xs[|xs| - 1] >= 1) then
                                 Success(Bitlist(fromBytesToBitList(xs)))
@@ -133,8 +192,7 @@ module SSZ {
      * Well typed deserialisation does not fail. 
      */
     lemma wellTypedDoesNotFail(s : Serialisable) 
-    requires || typeOf(s) in {Bool_,Bitlist_,Bytes32_}
-             || exists n:nat :: typeOf(s) == Uint_(n)
+    requires typeOf(s) in {Bool_, Uint8_, Uint16_, Uint32_, Uint64_, Uint128_, Uint256_, Bitlist_,Bytes32_}
         ensures deserialise(serialise(s), typeOf(s)) != Failure 
     {   //  Thanks Dafny.
     }
@@ -143,8 +201,7 @@ module SSZ {
      * Deserialise(serialise(-)) = Identity for well typed objects.
      */
     lemma seDesInvolutive(s : Serialisable) 
-        requires || typeOf(s) in {Bool_,Bitlist_,Bytes32_}
-                || exists n:nat :: typeOf(s) == Uint_(n)
+        requires typeOf(s) in {Bool_, Uint8_, Uint16_, Uint32_, Uint64_, Uint128_, Uint256_, Bitlist_,Bytes32_}
         ensures deserialise(serialise(s), typeOf(s)) == Success(s) 
         {   //  thanks Dafny.
             match s 
@@ -163,7 +220,19 @@ module SSZ {
 
                 case Bool(_) =>  //  Thanks Dafny
 
-                case Uint(_) => lemmaBytesToUintIsTheInverseOfUintToBytes(s);//  Thanks Dafny
+                case Uint8(_) => lemmaBytesToIntIsTheInverseOfIntToBytes(s.n8 as nat,1);
+
+                case Uint16(n) => lemmaBytesToIntIsTheInverseOfIntToBytes(s.n16 as nat,2);
+
+                case Uint32(n) => lemmaBytesToIntIsTheInverseOfIntToBytes(s.n32 as nat,4);
+
+                case Uint64(n) =>   UpperBoundForUint64(s.n64);
+                                    lemmaBytesToIntIsTheInverseOfIntToBytes(s.n64 as nat,8);
+
+                case Uint128(n) =>  assert 128 == 16 * 8;
+                                    lemmaBytesToIntIsTheInverseOfIntToBytes(s.n128 as nat,16);
+
+                case Uint256(n) => lemmaBytesToIntIsTheInverseOfIntToBytes(s.n256 as nat,32);
 
                 case Bytes32(_) => // Thanks Dafny
             
@@ -173,8 +242,7 @@ module SSZ {
      *  Serialise is injective.
      */
     lemma {:induction s1, s2} serialiseIsInjective(s1: Serialisable, s2 : Serialisable)
-        requires || typeOf(s1) in {Bool_,Bitlist_,Bytes32_}
-                 || exists n:nat :: typeOf(s1) == Uint_(n)
+        requires typeOf(s1) in {Bool_, Uint8_, Uint16_, Uint32_, Uint64_, Uint128_, Uint256_, Bitlist_,Bytes32_}
         ensures typeOf(s1) == typeOf(s2) ==> 
                     serialise(s1) == serialise(s2) ==> s1 == s2 
     {
