test/dafny/merkle/Merkleise.test.dfy
@@ -45,7 +45,7 @@ include "../../../src/dafny/merkle/Merkleise.dfy"
             TestItem(
                 "Count chunks for serialised uint8(5) is 1",
                 () => chunkCount(
-                    makeUint8(5 as uint8)
+                    Uint8(5 as uint8)
                     ) == 1 
             ),
             TestItem(
@@ -63,7 +63,7 @@ include "../../../src/dafny/merkle/Merkleise.dfy"
          var r2 := [
             TestItem(
                 "Right pad with zeros 127 has size 32",
-                () => |rightPadZeros(serialise(makeUint8(127)))| == 32 
+                () => |rightPadZeros(serialise(Uint8(127)))| == 32 
             )
             // TestItem(
             //     "Count chunks for serialised bool true is 1",
